Core/Metatheory/Uniqueness.lean
@@ -1,0 +1,61 @@
+import LeanSubst
+import Core.Term
+import Core.Reduction
+import Core.Typing
+import Core.Util
+
+import Core.Metatheory.Substitution
+import Core.Metatheory.Rename
+import Core.Metatheory.GlobalWf
+
+
+theorem Typing.spine_term_unique_typing :
+  G&Δ,Γ ⊢ a : A ->
+  G&Δ,Γ ⊢ a : T ->
+  a.spine = some (x, sp) ->
+  A = T := by
+intro j1 j2 h
+induction j1 generalizing T sp
+all_goals (try case _ h1 _ => cases j2; case _ h2 => rw[h1] at h2; cases h2; rfl)
+all_goals (try simp [Term.spine] at h)
+case _ b _ _ _ _ _ jf ja ih _ =>
+  cases b
+  all_goals (
+    simp [Term.spine] at *
+    rw[Option.bind_eq_some_iff] at h;
+    rcases h with ⟨w, h1, h2⟩
+    cases h2
+    cases j2; case _ h =>
+    have ih1 := ih h h1
+    have ih2 := ih jf h1
+    rw[ih1] at ih2
+    cases ih2; cases ih1; rfl
+  )
+case _ jf ja e ih =>
+  rw[Option.bind_eq_some_iff] at h
+  rcases h with ⟨w, h1, h2⟩
+  cases h2
+  cases j2; case _ h e' =>
+  have ih1 := ih h h1
+  have ih2 := ih jf h1
+  rw[ih1] at ih2
+  cases ih2; cases ih1
+  subst e'; subst e; rfl
+
+theorem Kinding.unique :
+  G&Δ ⊢ T : K ->
+  G&Δ ⊢ T : K' ->
+  K = K' := by
+intro j1 j2;
+induction j1 generalizing K'
+all_goals (try
+  case _ h1 =>
+    cases j2; case _ h2 =>
+    rw[h1] at h2; cases h2; rfl)
+all_goals (try
+  case _ => cases j2; rfl
+)
+case app jf ja ih1 ih2  =>
+  cases j2; case _ j1 j2 =>
+  replace ih2 := ih2 j1; cases ih2
+  replace ih1 := ih1 j2; cases ih1; rfl
